# baseURI: http://pervasive.semanticweb.org/ont/2019/07/consert/context-domain-org
# imports: http://www.w3.org/2019/td#

@prefix : <http://pervasive.semanticweb.org/ont/2019/07/consert/context-domain-org#> .
@prefix consert-core: <http://pervasive.semanticweb.org/ont/2017/07/consert/core#> .
@prefix owl: <http://www.w3.org/2002/07/owl#> .
@prefix rdf: <http://www.w3.org/1999/02/22-rdf-syntax-ns#> .
@prefix rdfs: <http://www.w3.org/2000/01/rdf-schema#> .
@prefix td: <https://www.w3.org/2019/wot/td#> .
@prefix xsd: <http://www.w3.org/2001/XMLSchema#> .

<http://pervasive.semanticweb.org/ont/2019/07/consert/context-domain-org>
  rdf:type owl:Ontology ;
  owl:imports <http://www.w3.org/2019/td#> ;
  owl:versionInfo "Created with TopBraid Composer"^^xsd:string ;
.
:ContextDimension
  rdf:type owl:Class ;
  rdfs:comment "The property/ContextAssertion which defines the dimension along which ContextDomain instances are created."^^xsd:string ;
  rdfs:label "ContextDimension"^^xsd:string ;
  rdfs:subClassOf owl:Thing ;
.
:ContextDomainEntity
  rdf:type owl:Class ;
  rdfs:comment "The range of a ContextDimension. Defines the class of ContextEntities which denote a ContextDomain (i.e. a common context denominator for producers and consumers of the context information from the domain.)."^^xsd:string ;
  rdfs:label "ContextDomain Entity"^^xsd:string ;
  rdfs:subClassOf owl:Thing ;
.
:ContextDomainGroup
  rdf:type owl:Class ;
  rdfs:comment "The group of context processing agents that share the context defined by a ContextDomain."^^xsd:string ;
  rdfs:label "ContextDomain Group"^^xsd:string ;
  rdfs:subClassOf owl:Thing ;
.
:ContextManagementAgent
  rdf:type owl:Class ;
  rdfs:comment "The generic class for logical units that manage context information."^^xsd:string ;
  rdfs:label "Context Management Agent"^^xsd:string ;
  rdfs:subClassOf owl:Thing ;
.
:CoordinatorAgent
  rdf:type owl:Class ;
  rdfs:comment "The agent centralizing and coordinating access to all context information of a ContextDomain."^^xsd:string ;
  rdfs:label "Coordinator Agent"^^xsd:string ;
  rdfs:subClassOf :ContextManagementAgent ;
.
:SensorAgent
  rdf:type owl:Class ;
  rdfs:comment "The agent managing sensor and actuator information."^^xsd:string ;
  rdfs:label "Sensor Agent"^^xsd:string ;
  rdfs:subClassOf :ContextManagementAgent ;
.
:UserAgent
  rdf:type owl:Class ;
  rdfs:comment "The agent issueing queries/subscriptions and actuation requests for sensors and actuators modeled in a ContextDomain."^^xsd:string ;
  rdfs:label "User Agent"^^xsd:string ;
  rdfs:subClassOf :ContextManagementAgent ;
.
:groupMemberOf
  rdf:type owl:ObjectProperty ;
  rdfs:comment "Property specifying the membership of a Context Management Agent to a ContextDomainGroup."^^xsd:string ;
  rdfs:domain :ContextManagementAgent ;
  rdfs:label "groupMemberOf"^^xsd:string ;
  rdfs:range :ContextDomainGroup ;
.
:hasDimension
  rdf:type owl:ObjectProperty ;
  rdfs:comment "Property relating a ContextDomainGroup and the ContextDimension it si a part of."^^xsd:string ;
  rdfs:domain :ContextDomainGroup ;
  rdfs:label "hasDimension"^^xsd:string ;
  rdfs:range :ContextDimension ;
.
:hasNature
  rdf:type owl:DatatypeProperty ;
  rdfs:comment "The nature of the ContextDimension, whether spatial, activity, relational or individual."^^xsd:string ;
  rdfs:label "hasNature"^^xsd:string ;
  rdfs:range [
      rdf:type rdfs:Datatype ;
      owl:oneOf (
          "spatial"^^xsd:string
          "activity"^^xsd:string
          "relational"^^xsd:string
          "individual"^^xsd:string
        ) ;
    ] ;
.
:managesThing
  rdf:type owl:ObjectProperty ;
  rdfs:comment "Property specifying the actuators/things that are managed by a SensorAgent."@en ;
  rdfs:domain :SensorAgent ;
  rdfs:label "managesThing"@en ;
  rdfs:range td:Thing ;
.
